ems/ModSemFacts.v
@@ -132,6 +132,43 @@ Section COMM.
   Lemma fst_trans_r : forall x, fst (trans_r x) = fst x.
   Proof. i. destruct x. ss. Qed.
 
+  Lemma fun_fst_trans_l : 
+    (fun x : string * (Any.t -> itree Es Any.t) => fst (trans_l x)) = (fun x : string * (Any.t -> itree Es Any.t) => fst x).
+  Proof.
+    extensionality x. rewrite fst_trans_l. et.
+  Qed.
+
+  Lemma fun_fst_trans_r : 
+    (fun x : string * (Any.t -> itree Es Any.t) => fst (trans_r x)) = (fun x : string * (Any.t -> itree Es Any.t) => fst x).
+  Proof.
+    extensionality x. rewrite fst_trans_r. et.
+  Qed.
+
+  Lemma fun_fst_trans_l_l :
+    (fun x : string * (Any.t -> itree Es Any.t) => fst (trans_l (trans_l x))) = (fun x : string * (Any.t -> itree Es Any.t) => fst x).
+  Proof.
+    extensionality x. rewrite ! fst_trans_l. et.
+  Qed.
+
+  Lemma fun_fst_trans_l_r :
+    (fun x : string * (Any.t -> itree Es Any.t) => fst (trans_l (trans_r x))) = (fun x : string * (Any.t -> itree Es Any.t) => fst x).
+  Proof.
+    extensionality x. rewrite fst_trans_l. rewrite fst_trans_r. et.
+  Qed.
+
+  Lemma fun_fst_trans_r_l:
+    (fun x : string * (Any.t -> itree Es Any.t) => fst (trans_r (trans_l x))) = (fun x : string * (Any.t -> itree Es Any.t) => fst x).
+  Proof.
+    extensionality x. rewrite fst_trans_r. rewrite fst_trans_l. et.
+  Qed.
+
+  Lemma fun_fst_trans_r_r:
+    (fun x : string * (Any.t -> itree Es Any.t) => fst (trans_r (trans_r x))) = (fun x : string * (Any.t -> itree Es Any.t) => fst x).
+  Proof.
+    extensionality x. rewrite ! fst_trans_r. et.
+  Qed.
+
+
   Context {CONF: EMSConfig}.
 
   Theorem add_comm
@@ -150,7 +187,7 @@ Section COMM.
     - i. s.
       unfold add_fnsems. rewrite ! alist_find_app_o.
       destruct (alist_find fn (fnsems ms1)) eqn:MS1; destruct (alist_find fn (fnsems ms0)) eqn: MS0.
-      + right. right. unfold trans_l.
+      + right. unfold trans_l.
         exists (fun args => translate emb_l (i args)).
         exists (fun args => translate emb_r (i args)).
         rewrite ! alist_find_map.
@@ -161,17 +198,15 @@ Section COMM.
           apply NoDup_app_disjoint with (a:=fn) in wf_fnsems0.
           -- clarify.
           -- replace fn with (fst (fn, i)); et.
-             replace (fun x : string * (Any.t -> itree Es Any.t) => fst (trans_l x)) with (fun x : string * (Any.t -> itree Es Any.t) => fst x).
-             2: { extensionality x. rewrite fst_trans_l. et. }
+             rewrite fun_fst_trans_l.
              apply in_map. apply alist_find_some in MS1. et. 
           -- replace fn with (fst (fn, i0)); et.
-             replace (fun x : string * (Any.t -> itree Es Any.t) => fst (trans_r x)) with (fun x : string * (Any.t -> itree Es Any.t) => fst x).
-             2: { extensionality x. rewrite fst_trans_r. et. }
+             rewrite fun_fst_trans_r.
              apply in_map. apply alist_find_some in MS0. et.
         * instantiate (1:= top2). instantiate (1:= unit). instantiate (1:=(fun _ => comm_st)).
           unfold sim_fsem, "==>". i. eapply add_comm_aux; et.
           rewrite H0. econs. econs.
-      + right. right. unfold trans_l.
+      + right. unfold trans_l.
         exists (fun args => translate emb_l (i args)).
         exists (fun args => translate emb_r (i args)).          
         rewrite ! alist_find_map.
@@ -182,7 +217,7 @@ Section COMM.
         * unfold sim_fsem, "==>". i. eapply add_comm_aux; et.
           rewrite H0. econs. econs.
 
-      + right. right. unfold trans_l.
+      + right. unfold trans_l.
         exists (fun args => translate emb_r (i args)).
         exists (fun args => translate emb_l (i args)).          
         rewrite ! alist_find_map.
@@ -441,39 +476,33 @@ Proof.
     rewrite ! List.map_app in *. rewrite ! List.map_map in *.
     apply NoDup_app_disjoint with (a:=fn) in wf_fnsems0; ss.
     + replace fn with (fst (fn, i)); et.
-      replace (fun x : string * (Any.t -> itree Es Any.t) => fst (trans_l x)) with (fun x : string * (Any.t -> itree Es Any.t) => fst x).
-      2: { extensionality x. rewrite fst_trans_l. et. }
+      rewrite fun_fst_trans_l.
       apply in_map. apply alist_find_some in MS0. et.
     + replace fn with (fst (fn, i0)); et.
-      replace (fun x : string * (Any.t -> itree Es Any.t) => fst (trans_r (trans_l x))) with (fun x : string * (Any.t -> itree Es Any.t) => fst x).
-      2: { extensionality x. rewrite fst_trans_r. rewrite fst_trans_l. et. }
+      rewrite fun_fst_trans_r_l.
       apply in_app_iff. left. 
       apply in_map. apply alist_find_some in MS1. et.
   - inv WF. ss. unfold add_fnsems in wf_fnsems0. ss. unfold add_fnsems in wf_fnsems0.
     rewrite ! List.map_app in *. rewrite ! List.map_map in *.
     apply NoDup_app_disjoint with (a:=fn) in wf_fnsems0; ss.
     + replace fn with (fst (fn, i)); et.
-      replace (List.map (fun x : string * (Any.t -> itree Es Any.t) => fst (trans_l x))) with (List.map (fun x : string * (Any.t -> itree Es Any.t) => fst x)).
-      2: { f_equal. extensionality x. rewrite fst_trans_l. et. }
+      rewrite fun_fst_trans_l.
       apply in_map. apply alist_find_some in MS0. et.
     + replace fn with (fst (fn, i0)); et.
-      replace (fun x : string * (Any.t -> itree Es Any.t) => fst (trans_r (trans_l x))) with (fun x : string * (Any.t -> itree Es Any.t) => fst x).
-      2: { extensionality x. rewrite fst_trans_r. rewrite fst_trans_l. et. }
+      rewrite fun_fst_trans_r_l.
       apply in_app_iff. left. apply in_map.
       apply alist_find_some in MS1. et.
   - inv WF. ss. unfold add_fnsems in wf_fnsems0. ss. unfold add_fnsems in wf_fnsems0.
     rewrite ! List.map_app in *. rewrite ! List.map_map in *.
     apply NoDup_app_disjoint with (a:=fn) in wf_fnsems0; ss.
     + replace fn with (fst (fn, i)); et.
-      replace (List.map (fun x : string * (Any.t -> itree Es Any.t) => fst (trans_l x))) with (List.map (fun x : string * (Any.t -> itree Es Any.t) => fst x)).
-      2: { f_equal. extensionality x. rewrite fst_trans_l. et. }
+      rewrite fun_fst_trans_l.
       apply in_map. apply alist_find_some in MS0. et.
     + replace fn with (fst (fn, i0)); et.
-      replace (fun x : string * (Any.t -> itree Es Any.t) => fst (trans_r (trans_r x))) with (fun x : string * (Any.t -> itree Es Any.t) => fst x).
-      2: { extensionality x. rewrite fst_trans_r. rewrite fst_trans_r. et. }
+      rewrite fun_fst_trans_r_r.
       apply in_app_iff. right. apply in_map.
       apply alist_find_some in MS2. et.
-  - right. right. esplits; et; s; et.
+  - right. esplits; et; s; et.
     unfold sim_fsem, "==>". i. eapply add_assoc_aux; et.
     rewrite H0. 
     erewrite <- (@bisimulation_is_eq _ _ _ _ (@translate_cmpE _ _ _ _ _ _ _)).
@@ -483,20 +512,18 @@ Proof.
     rewrite List.app_assoc in *.
     apply NoDup_app_disjoint with (a:=fn) in wf_fnsems0; ss.
     + replace fn with (fst (fn, i)); et.
-      replace (List.map (fun x : string * (Any.t -> itree Es Any.t) => fst (trans_r (trans_l x)))) with (List.map (fun x : string * (Any.t -> itree Es Any.t) => fst x)).
-      2: { f_equal. extensionality x. rewrite fst_trans_r. rewrite fst_trans_l. et. }
+      rewrite fun_fst_trans_r_l.
       apply in_app_iff. right. 
       apply in_map. apply alist_find_some in MS1. et.
     + replace fn with (fst (fn, i0)); et.
-      replace (fun x : string * (Any.t -> itree Es Any.t) => fst (trans_r (trans_r x))) with (fun x : string * (Any.t -> itree Es Any.t) => fst x).
-      2: { extensionality x. rewrite fst_trans_r. rewrite fst_trans_r. et. }
+      rewrite fun_fst_trans_r_r.
       apply in_map. apply alist_find_some in MS2. et.
-  - right. right. esplits; et; s; et.
+  - right. esplits; et; s; et.
     unfold sim_fsem, "==>". i. eapply add_assoc_aux; et.
     rewrite H0.
     erewrite <- ! (@bisimulation_is_eq _ _ _ _ (@translate_cmpE _ _ _ _ _ _ _)).
     econs. econs.
-  - right. right. esplits; et; s; et.
+  - right. esplits; et; s; et.
     unfold sim_fsem, "==>". i. eapply add_assoc_aux; et.
     rewrite H0.
     erewrite <- ! (@bisimulation_is_eq _ _ _ _ (@translate_cmpE _ _ _ _ _ _ _)).
@@ -529,7 +556,7 @@ Proof.
   destruct (alist_find fn (fnsems ms0)) eqn: MS0; 
   destruct (alist_find fn (fnsems ms1)) eqn:MS1; 
   destruct (alist_find fn (fnsems ms2)) eqn: MS2;
-  ( ss; et; right; right; esplits; et; s; et; unfold sim_fsem, "==>"; i; eapply add_assoc_rev_aux; et; rewrite H0;
+  ( ss; et; right; esplits; et; s; et; unfold sim_fsem, "==>"; i; eapply add_assoc_rev_aux; et; rewrite H0;
     erewrite <- ! (@bisimulation_is_eq _ _ _ _ (@translate_cmpE _ _ _ _ _ _ _)); econs; econs).
 Qed.
 
@@ -549,6 +576,12 @@ Definition empty_st (stp: Any.t * Any.t) : Prop :=
   exists a, fst stp = a /\ 
   snd stp = Any.pair a tt↑
 .
+
+Definition empty_rev_st (stp: Any.t * Any.t) : Prop :=
+  exists a, fst stp = Any.pair a tt↑ /\ 
+  snd stp = a
+.
+
 
 Lemma add_empty_aux
         itl itr stl str (w: unit)
@@ -613,6 +646,69 @@ Proof.
 
 Qed.
 
+Lemma add_empty_rev_aux
+        itl itr stl str (w: unit)
+        (EMPTY: empty_ems itr itl)
+        (STATE: empty_rev_st (stl, str))
+
+  :
+      sim_itree (fun _ => empty_rev_st) top2 false false w (stl, itl) (str, itr)
+.
+Proof.
+  destruct EMPTY, STATE. des. ss.
+  unfold empty_rev_st.
+  ginit. 
+  generalize it as itr. 
+  clarify.
+  generalize x as a.
+  gcofix CIH. i.
+  ides itr.
+  - (* Ret *)
+    erewrite ! (bisimulation_is_eq _ _ (translate_ret _ _)).
+    gstep. apply sim_itree_ret.
+    unfold lift_rel. 
+    exists tt. splits; et. exists a. ss.
+  - (* Tau *)
+    erewrite ! (bisimulation_is_eq _ _ (translate_tau _ _)).
+    gstep. 
+    apply sim_itree_tau_src. apply sim_itree_tau_tgt. 
+    eapply sim_itree_progress; et.
+    gfinal. left. eapply CIH; et.
+  - (* Vis *)
+    erewrite ! (bisimulation_is_eq _ _ (translate_vis _ _ _ _)).
+    rewrite <- ! bind_trigger.
+    destruct e as [c|[s|e]].
+    + (* callE *)
+      gstep. destruct c, EMB. 
+      apply sim_itree_call; clarify.
+      -- exists a; et.
+      -- i. destruct WF, H. ss. clarify.
+         gfinal. left. eapply CIH.
+    + (* sE *)
+      gstep. destruct s, EMB.
+      apply sim_itree_supdate_src. apply sim_itree_supdate_tgt.
+      eapply sim_itree_progress; et.
+      unfold run_l, run_r. rewrite ! Any.pair_split.
+      gfinal. left. destruct (run a). eapply CIH.
+      
+    + (* eventE *)
+      gstep. destruct e, EMB.
+      (* Choose *)
+      * apply sim_itree_choose_tgt. i. apply sim_itree_choose_src. exists x0.
+        eapply sim_itree_progress; et.
+        gfinal. left. eapply CIH.
+      (* Take *)
+        * apply sim_itree_take_src. i. apply sim_itree_take_tgt. exists x0.
+        eapply sim_itree_progress; et.
+        gfinal. left. eapply CIH. 
+      (* Syscall *)
+        * apply sim_itree_syscall. i.
+        eapply sim_itree_flag_down.
+        gfinal. left. eapply CIH. 
+
+Qed.
+
+
 Context {CONF: EMSConfig}.
 
 Theorem add_empty
@@ -637,11 +733,39 @@ Proof.
   rewrite ! alist_find_app_o. rewrite ! alist_find_map. 
   destruct (alist_find fn (fnsems ms)) eqn: MS; cycle 1.
   - left. et.
-  - ss. right. right. esplits; et.
+  - ss. right. esplits; et.
     unfold sim_fsem, "==>". i. apply add_empty_aux; et.
     rewrite H0. econs. econs.
 Qed.
+
+Theorem add_empty_rev
+      ms
+      (P0 P1: Prop) (IMPL: P1 -> P0)
+      (WF: wf ms)
+:
+  <<EMPTY: Beh.of_program (compile ms (Some P0)) <1=
+          Beh.of_program (compile (add ms empty) (Some P1))>>
+.
+Proof. 
+  destruct (classic (P1)); cycle 1.
+  { ii. eapply initial_itr_not_wf;et. }
+  replace P0 with P1.
+  2: { eapply prop_ext. split; auto. }
+  unfold compile. red. 
+  eapply adequacy_local_aux; et.
+  2: { exists tt. instantiate (1:= top2). instantiate (1:= (fun _ => empty_rev_st)). econs; et; clarify.
+       unfold empty_st. ss. exists (init_st ms). et. }
+  i. s.
+  unfold add_fnsems, trans_l, trans_r. s.
+  rewrite ! alist_find_app_o. rewrite ! alist_find_map. 
+  destruct (alist_find fn (fnsems ms)) eqn: MS; cycle 1.
+  - left. et.
+  - ss. right. esplits; et.
+    unfold sim_fsem, "==>". i. apply add_empty_rev_aux; et.
+    rewrite H0. econs. econs.
+Qed.
 End EMPTY.
+
 
 End ModSemFacts.
 
@@ -660,84 +784,76 @@ Theorem add_comm
 .
 
 Proof.
-ii. unfold compile in *.
-destruct (classic (ModSem.wf (enclose (add md1 md0)) /\ Sk.wf (sk (add md1 md0)))).
-2: { eapply ModSem.initial_itr_not_wf. ss. }
-ss. des. assert (SK: Sk.wf (Sk.add (sk md0) (sk md1))).
-{ apply Sk.wf_comm. auto. }
-rewrite Sk.add_comm; et.
-eapply ModSemFacts.add_comm; [| |et].
-{ i. split; auto. unfold enclose. ss. rewrite Sk.add_comm; et.
-  inv H2. inv H3. econs; ss.
-  unfold ModSem.add_fnsems in *.
-  rewrite ! List.map_app in *.
-  rewrite ! List.map_map in *.
-  replace (fun x : string * (Any.t -> itree Es Any.t) => fst (ModSem.trans_l x)) with (fun x : string * (Any.t -> itree Es Any.t) => fst x) in *.
-  2: { extensionality x. rewrite ModSemFacts.fst_trans_l. et. }
-  replace (fun x : string * (Any.t -> itree Es Any.t) => fst (ModSem.trans_r x)) with (fun x : string * (Any.t -> itree Es Any.t) => fst x) in *.
-  2: { extensionality x. rewrite ModSemFacts.fst_trans_r. et. }
-  eapply nodup_comm. et.
-}
-{ rewrite Sk.add_comm; et. }
+  ii. unfold compile in *.
+  destruct (classic (ModSem.wf (enclose (add md1 md0)) /\ Sk.wf (sk (add md1 md0)))).
+  2: { eapply ModSem.initial_itr_not_wf. ss. }
+  ss. des. assert (SK: Sk.wf (Sk.add (sk md0) (sk md1))).
+  { apply Sk.wf_comm. auto. }
+  rewrite Sk.add_comm; et.
+  eapply ModSemFacts.add_comm; [| |et].
+  { i. split; auto. unfold enclose. ss. rewrite Sk.add_comm; et.
+    inv H2. inv H3. econs; ss.
+    unfold ModSem.add_fnsems in *.
+    rewrite ! List.map_app in *.
+    rewrite ! List.map_map in *.
+    rewrite ModSemFacts.fun_fst_trans_l in *.
+    rewrite ModSemFacts.fun_fst_trans_r in *.
+    eapply nodup_comm. et.
+  }
+  { rewrite Sk.add_comm; et. }
 Qed.
-
-
-(* Lemma add_assoc' ms0 ms1 ms2:
-  add ms0 (add ms1 ms2) = add (add ms0 ms1) ms2.
-Proof.
-  unfold add. f_equal.
-  { extensionality skenv_link. ss. apply ModSem.add_assoc'. }
-  { ss. rewrite Sk.add_assoc. auto. }
-Qed. *)
 
 Theorem add_assoc
         md0 md1 md2
   :
-    <<ASSOC: Beh.of_program (compile (add md0 (add md1 md2))) <1=
-            Beh.of_program (compile (add (add md0 md1) md2))>>
+    <<ASSOC: Beh.of_program (compile (add (add md0 md1) md2)) <1=
+            Beh.of_program (compile (add md0 (add md1 md2)))>>
 .
 Proof. 
-ii. unfold compile in *.
-destruct (classic (ModSem.wf (enclose (add (add md0 md1) md2)) /\ Sk.wf (sk (add (add md0 md1) md2)))).
-2: { eapply ModSem.initial_itr_not_wf. ss. }
-ss. des. assert (SK: Sk.wf (Sk.add (sk md0) (Sk.add (sk md1) (sk md2)))).
-{ rewrite Sk.add_assoc. apply H1. }
-
-Search Sk.t.
-
-(* Sk associativity required *)
-
-{ admit. }
-Admitted.
-(* 
-rewrite Sk.sort_add_assoc; et.
-eapply ModSemFacts.add_comm; [| |et].
-{ i. split; auto. unfold enclose. ss. rewrite Sk.sort_add_comm; et.
-  inv H1. inv H2. econs; ss.
-  unfold ModSem.add_fnsems in *.
-  rewrite ! List.map_app in *.
-  rewrite ! List.map_map in *.
-  replace (fun x : string * (Any.t -> itree Es Any.t) => fst (ModSem.trans_l x)) with (fun x : string * (Any.t -> itree Es Any.t) => fst x) in *.
-  2: { extensionality x. rewrite ModSemFacts.fst_trans_l. et. }
-  replace (fun x : string * (Any.t -> itree Es Any.t) => fst (ModSem.trans_r x)) with (fun x : string * (Any.t -> itree Es Any.t) => fst x) in *.
-  2: { extensionality x. rewrite ModSemFacts.fst_trans_r. et. }
-  eapply nodup_comm. et.
-}
-{ rewrite Sk.sort_add_comm; et. }
-
- *)
-
-(* Qed. *)
+  ii. unfold compile in *.
+  destruct (classic (ModSem.wf (enclose (add md0 (add md1 md2))) /\ Sk.wf (sk (add md0 (add md1 md2))))).
+  2: { eapply ModSem.initial_itr_not_wf. ss. }
+  ss. des. assert (SK: Sk.wf (Sk.add (Sk.add (sk md0) (sk md1)) (sk md2))).
+  { rewrite <- Sk.add_assoc. apply H1. }
+  eapply ModSemFacts.add_assoc; [ |et|rewrite Sk.add_assoc;et].
+  i. split; et. unfold enclose. ss.
+  rewrite <- Sk.add_assoc.
+  inv H2. inv H3. econs.
+  repeat (ss; unfold ModSem.add_fnsems in *; rewrite ! List.map_app in *; rewrite ! List.map_map in *).
+  rewrite ModSemFacts.fun_fst_trans_l in *.
+  rewrite ModSemFacts.fun_fst_trans_r in *.
+  rewrite ModSemFacts.fun_fst_trans_l_l in *.
+  rewrite ModSemFacts.fun_fst_trans_l_r in *.
+  rewrite ModSemFacts.fun_fst_trans_r_l in *.
+  rewrite ModSemFacts.fun_fst_trans_r_r in *.
+  rewrite <- app_assoc. apply wf_fnsems.
+Qed.
 
 Theorem add_assoc_rev
         md0 md1 md2
   :
-    <<COMM: Beh.of_program (compile (add (add md0 md1) md2)) <1=
-            Beh.of_program (compile (add md0 (add md1 md2)))>>
+    <<COMM: Beh.of_program (compile (add md0 (add md1 md2))) <1=
+            Beh.of_program (compile (add (add md0 md1) md2))>>
 .
-Proof. Admitted.
-  (* rewrite add_assoc'. ss.
-Qed. *)
+Proof.
+  ii. unfold compile in *.
+  destruct (classic (ModSem.wf (enclose (add (add md0 md1) md2)) /\ Sk.wf (sk (add (add md0 md1) md2)))).
+  2: { eapply ModSem.initial_itr_not_wf. ss. }
+  ss. des. assert (SK: Sk.wf (Sk.add (sk md0) (Sk.add (sk md1) (sk md2)))).
+  { rewrite Sk.add_assoc. apply H1. }
+  eapply ModSemFacts.add_assoc_rev; [ |et|rewrite <- Sk.add_assoc;et].
+  i. split; et. unfold enclose. ss.
+  rewrite Sk.add_assoc.
+  inv H2. inv H3. econs.
+  repeat (ss; unfold ModSem.add_fnsems in *; rewrite ! List.map_app in *; rewrite ! List.map_map in *).
+  rewrite ModSemFacts.fun_fst_trans_l in *.
+  rewrite ModSemFacts.fun_fst_trans_r in *.
+  rewrite ModSemFacts.fun_fst_trans_l_l in *.
+  rewrite ModSemFacts.fun_fst_trans_l_r in *.
+  rewrite ModSemFacts.fun_fst_trans_r_l in *.
+  rewrite ModSemFacts.fun_fst_trans_r_r in *.
+  rewrite app_assoc. apply wf_fnsems.
+Qed.
 
 Lemma add_empty_r 
       md
@@ -746,26 +862,24 @@ Lemma add_empty_r
               Beh.of_program (compile md)>>
 .
 Proof.
-ii. unfold compile in *.
-destruct (classic (ModSem.wf (enclose md) /\ Sk.wf (sk md))).
-2: { eapply ModSem.initial_itr_not_wf. ss. }
-ss. des. assert (SK: Sk.wf (Sk.add (sk md) Sk.unit)).
-{ rewrite Sk.add_unit_r. et.  }
-eapply ModSemFacts.add_empty; [|et|].
-- instantiate (1:= wf (add md empty)). i.
-  unfold wf. esplits; et. ss.
-  inv H0. econs. 
-  rewrite Sk.add_unit_r.
-  unfold ModSem.add, ModSem.add_fnsems. ss.
-  rewrite List.map_app. rewrite List.map_map.
-  ss. rewrite app_nil_r.
-  replace (fun x : string * (Any.t -> itree Es Any.t) => fst (ModSem.trans_l x)) with ((fun x : string * (Any.t -> itree Es Any.t) => fst x)).
-  2: { extensionality x. rewrite ModSemFacts.fst_trans_l. et. }
-  ss.
-  
-- unfold ModSem.compile, ModSem.empty, enclose.
-  rewrite Sk.add_unit_r in PR. et.
-  
+  ii. unfold compile in *.
+  destruct (classic (ModSem.wf (enclose md) /\ Sk.wf (sk md))).
+  2: { eapply ModSem.initial_itr_not_wf. ss. }
+  ss. des. assert (SK: Sk.wf (Sk.add (sk md) Sk.unit)).
+  { rewrite Sk.add_unit_r. et.  }
+  eapply ModSemFacts.add_empty; [|et|].
+  - instantiate (1:= wf (add md empty)). i.
+    unfold wf. esplits; et. ss.
+    inv H0. econs. 
+    rewrite Sk.add_unit_r.
+    unfold ModSem.add, ModSem.add_fnsems. ss.
+    rewrite List.map_app. rewrite List.map_map.
+    ss. rewrite app_nil_r.
+    rewrite ModSemFacts.fun_fst_trans_l.
+    ss.
+
+  - unfold ModSem.compile, ModSem.empty, enclose.
+    rewrite Sk.add_unit_r in PR. et.
 Qed.
 
 Lemma add_empty_l 
@@ -774,9 +888,56 @@ Lemma add_empty_l
     << EMPTY: Beh.of_program (compile (add empty md)) <1=
               Beh.of_program (compile md)>>
 .
+Proof.
+  ii. apply add_empty_r. apply add_comm. et.
+Qed.
+
+Lemma add_empty_rev_r
+      md
+  : 
+    << EMPTY: Beh.of_program (compile md) <1=
+              Beh.of_program (compile (add md empty))>>
+.
+Proof.
+  ii. unfold compile in *.
+  destruct (classic (ModSem.wf (enclose (add md empty)) /\ Sk.wf (sk (add md empty)))).
+  2: { eapply ModSem.initial_itr_not_wf. ss. }
+  des. assert (SK: Sk.wf (sk md)).
+  { ss. rewrite Sk.add_unit_r in H1. et.  }
+
+  eapply ModSemFacts.add_empty_rev.
+  
+  2: { ss. rewrite Sk.add_unit_r in *. inv H0. econs. 
+       unfold ModSem.add in wf_fnsems. ss.
+       unfold ModSem.add_fnsems in wf_fnsems. ss.
+       rewrite List.map_app in wf_fnsems.
+       rewrite List.map_map in wf_fnsems.
+       rewrite ModSemFacts.fun_fst_trans_l in wf_fnsems. ss.
+       eapply nodup_app_l in wf_fnsems. ss. }
+  - instantiate (1:= wf md). i.
+    unfold wf. esplits; et. ss.
+    inv H0. econs. 
+    rewrite Sk.add_unit_r in wf_fnsems.
+    unfold ModSem.add, ModSem.add_fnsems in *. ss.
+    rewrite List.map_app, List.map_map in wf_fnsems.
+    ss. rewrite app_nil_r in wf_fnsems.
+    rewrite ModSemFacts.fun_fst_trans_l in wf_fnsems.
+    ss.
+
+  - unfold ModSem.compile, ModSem.empty, enclose. ss.
+    rewrite Sk.add_unit_r. et.
+Qed.
+
+Lemma add_empty_rev_l
+      md
+  : 
+    << EMPTY: Beh.of_program (compile md) <1=
+              Beh.of_program (compile (add empty md))>>
+.
 Proof. 
-(* empty_r + comm *)
-Admitted.
+  ii. apply add_comm. apply add_empty_rev_r. et. 
+Qed.
+
 
 
 (* Do we still add by list? (and refines2, refines_proper, etc.)
@@ -815,7 +976,6 @@ Section REFINE.
   Section CONF.
   Context {CONF: EMSConfig}.
 
-  
   (*** vertical composition ***)
   Global Program Instance refines_PreOrder: PreOrder refines.
 
@@ -845,12 +1005,39 @@ Section REFINE.
     pose proof ModFacts.add_assoc as ASSOC. 
     pose proof ModFacts.add_assoc_rev as ASSOC'. 
     r in COMM. r in ASSOC. r in ASSOC'.
-    apply ASSOC'. 
+    apply ASSOC. 
     apply SIM1.
-    apply ASSOC. apply COMM. apply ASSOC. apply COMM.
+    apply ASSOC'. apply COMM. apply ASSOC'. apply COMM.
     apply SIM0.
-    apply ASSOC. apply COMM. apply ASSOC.
+    apply ASSOC'. apply COMM. apply ASSOC'.
     apply PR.
+  Qed.
+
+  Theorem refines_proper_l
+    (mds0_src mds0_tgt: list Mod.t) (ctx: Mod.t)
+    (SIM0: refines (Mod.add_list mds0_tgt) (Mod.add_list mds0_src))
+  :
+    <<SIM: refines (Mod.add ctx (Mod.add_list mds0_tgt)) (Mod.add ctx (Mod.add_list mds0_src))>>
+  .
+  Proof.
+    ii. r in SIM0.
+    apply ModFacts.add_assoc. apply ModFacts.add_assoc_rev in PR.
+    apply SIM0. apply PR. 
+  Qed.
+
+  Theorem refines_proper_r
+    (mds0_src mds0_tgt: list Mod.t) (ctx: Mod.t)
+    (SIM0: refines (Mod.add_list mds0_tgt) (Mod.add_list mds0_src))
+  :
+    <<SIM: refines (Mod.add (Mod.add_list mds0_tgt) (ctx)) (Mod.add (Mod.add_list mds0_src) (ctx))>>
+  .
+  Proof.
+    ii. r in SIM0.
+    pose proof ModFacts.add_comm as COMM.
+    apply COMM. apply COMM in PR.
+    apply ModFacts.add_assoc_rev. apply ModFacts.add_assoc in PR.
+    apply COMM. apply COMM in PR.
+    apply SIM0. apply PR.  
   Qed.
 
   Lemma refines_close: refines <2= refines_closed.
@@ -859,9 +1046,9 @@ Section REFINE.
     pose proof ModFacts.add_empty_l as EMP.
     r in EMP.
     apply EMP with (x0 := x2) in PR.
-    2: { admit. (* empty_rev required. *) } 
+    2: { apply ModFacts.add_empty_rev_l. et. } 
     apply PR.
-  Admitted.
+  Qed.
 
   End CONF.
 
