ems/SImModSemFacts.v
@@ -23,258 +23,124 @@ Require Import ModSemFacts.
 Import TAC.
 
 Section ADEQUACY.
+  (* Context {CONF: EMSConfig}. *)
 
-  Definition embl_st (stp: Any.t * Any.t) : Prop :=
-    exists a b c, (fst stp = Any.pair a b /\ 
-    snd stp = Any.pair a c).
+  Lemma sim_ctx_mod
+    ctx md1 md2
+    (SIM: ModPair.sim md1 md2)
 
-  Lemma sim_emb_l 
-    x x' (wf: unit -> Any.t * Any.t -> Prop) wf' (w:unit) it
-    (WF: wf tt (x, x'))
-    (WF': wf' = (fun _ '(stl, str) => match (Any.split stl), (Any.split str) with
-                                      | Some (xl, _), Some (xr, _) => wf tt (xl, xr)
-                                      | _, _ => False
-                                      end
-    ) )
-    (* (SIM: sim_itree wf top2 false false w (x, it) (x', it)) *)
-    (SIM: sim_fsem wf top2 (fun _ => it) (fun _ => it))
   :
-    forall x1 x2, sim_itree wf' top2 false false w (Any.pair x x1, translate ModSem.emb_l it)
-    (Any.pair x' x2, translate ModSem.emb_l it)
+    ModPair.sim (Mod.add ctx md1) (Mod.add ctx md2)
   .
   Proof.
-    ginit. 
-    generalize it as itr.
-    revert WF. 
-    generalize x as a.
-    generalize x' as b.
-    gcofix CIH. i.
-    rewrite (itree_eta_ itr).
-    destruct (observe itr).
-    - (* Ret *)
-    erewrite ! (bisimulation_is_eq _ _ (translate_ret _ _)).
-    gstep. apply sim_itree_ret.
-    unfold lift_rel. 
-    exists w. splits; et. rewrite WF'. rewrite ! Any.pair_split. et.
-  - (* Tau *)
-    erewrite ! (bisimulation_is_eq _ _ (translate_tau _ _)).
-    gstep. 
-    apply sim_itree_tau_src. apply sim_itree_tau_tgt. 
-    eapply sim_itree_progress; et.
-    gfinal. left. eapply CIH; et.
-  - (* Vis *)
-    erewrite ! (bisimulation_is_eq _ _ (translate_vis _ _ _ _)).
-    rewrite <- ! bind_trigger.
-    destruct e as [c|[s|e']].
-    + (* callE *)
-      gstep. destruct c.
-      eapply sim_itree_call; clarify.
-      -- rewrite ! Any.pair_split. apply WF.
-      -- i. des_ifs. 
-         gfinal. left. apply Any.split_pair in Heq. apply Any.split_pair in Heq0.
-         des. clarify. eapply CIH. apply WF0.
-    + (* sE *)
-      gstep. destruct s.
-      apply sim_itree_supdate_src. apply sim_itree_supdate_tgt.
-      eapply sim_itree_progress; et.
-      unfold ModSem.run_l. rewrite ! Any.pair_split.
-      gfinal. left. destruct (run a), (run b). ss. eapply CIH.
-      
-    + (* eventE *)
-      gstep. destruct e, EMB.
-      (* Choose *)
-      * apply sim_itree_choose_tgt. i. apply sim_itree_choose_src. exists x0.
-        eapply sim_itree_progress; et.
-        gfinal. left. eapply CIH.
-      (* Take *)
-        * apply sim_itree_take_src. i. apply sim_itree_take_tgt. exists x0.
-        eapply sim_itree_progress; et.
-        gfinal. left. eapply CIH. 
-      (* Syscall *)
-        * apply sim_itree_syscall. i.
-        eapply sim_itree_flag_down.
-        gfinal. left. eapply CIH. 
-  Admitted.
+    inv SIM.
+    econs; et.
+    - i. ss. hexploit (sim_modsem sk); et.
+      2: { ii. des. apply sim_ctx. apply H. }
+      unfold Sk.incl, Sk.add in *. i. ss.
+      apply SKINCL.
+      rewrite in_app_iff. et.
+    - r. ss. unfold Sk.add. ss.
+      rewrite sim_sk. et.
+  Qed.
+
+  Lemma adequacy_mod
+          md_src md_tgt
+          (CONF: EMSConfig)
+          (SIM: ModPair.sim md_src md_tgt)
+    :
+    <<REF: Beh.of_program (Mod.compile md_tgt) <1= Beh.of_program (Mod.compile md_src) >>
+    .
+  Proof.
+    ii. unfold Mod.compile in *.
+    destruct (classic (ModSem.wf (Mod.enclose (md_src)) /\ Sk.wf (Mod.sk md_src))).
+    2: { eapply ModSem.initial_itr_not_wf. ss. }
+    ss. des. 
+    pose (sk_tgt := (Mod.sk (md_tgt))).
+    pose (sk_src := (Mod.sk (md_src))).
+    assert (SKEQ: sk_src = sk_tgt).
+    { unfold sk_tgt, sk_src. inv SIM. et. }
+    unfold Mod.enclose in *. fold sk_src in H. inv H.
+    inv SIM. hexploit (sim_modsem (Sk.canon sk_tgt)).
+    { etrans; [|eapply Sk.sort_incl]. ss. }
+    { ss. rewrite sim_sk in H0.
+      clear - H0.
+      unfold Sk.wf in *. ss.
+      eapply Permutation.Permutation_NoDup; [|et].
+      eapply Permutation.Permutation_map.
+      eapply Sk.SkSort.sort_permutation. }
+    i. des.
+    inv H. ss.
+
+    assert (WFTGT: Mod.wf md_tgt).
+    { rr. unfold Mod.enclose. ss. fold sk_tgt. 
+      rewrite SKEQ in *. split; auto.
+      2: { rewrite <-SKEQ. unfold sk_src. et. }
+      econs.
+      match goal with
+        | H: NoDup ?l0 |- NoDup ?l1 => replace l1 with l0
+      end; auto.
+      eapply Forall2_eq. eapply Forall2_apply_Forall2; et.
+      i. destruct a, b. inv H. ss.
+    }
+
+    eapply adequacy_local_aux in PR; et.
+    - i. esplits.
+      pose (ms_src := Mod.get_modsem md_src (Sk.sort (Mod.sk md_src))).
+      pose (ms_tgt := Mod.get_modsem md_tgt (Sk.sort (Mod.sk md_tgt))).
+      fold ms_src ms_tgt.
+      rewrite <- SKEQ in sim_fnsems at 1.
+      unfold sk_src, sk_tgt in sim_fnsems.
+      fold ms_src ms_tgt in sim_fnsems.
+      hexploit sim_fnsems. i.
+
+      destruct (alist_find fn (ModSem.fnsems ms_src)) eqn:SRC; destruct (alist_find fn (ModSem.fnsems ms_tgt)) eqn:TGT; et.
+      2: {
+        eapply alist_find_some in SRC.
+        (* eapply alist_find_none in TGT. *)
+        eapply Forall2_In_l with (a:= (fn, i)) in sim_fnsems; et.
+        inv sim_fnsems. inv H1.
+        inv H3. inv H1.
+        destruct x. ss. clarify.
+        apply alist_find_none with (v:=i0) in TGT. clarify. 
+      }
+      right. esplits; et.
+
+      hexploit SRC. hexploit TGT. i.
+      apply alist_find_some in H1, H2.
+
+      eapply Forall2_In_l with (a:=(fn, i)) in sim_fnsems; et.
+      eapply Forall2_In_r with (b:=(fn, i0)) in H; et.
+      inv sim_fnsems. inv H.
+      destruct x, x1.
+      inv H3. inv H5. inv H3. ss.
+      inv H4. inv H7. inv H4. ss. clarify.
+      unfold "@@2" in H5, H6. ss.
+      (* apply NoDup_map_inv in wf_fnsems. *)
+      unfold sk_src in wf_fnsems.
+      fold ms_src in wf_fnsems.
+      eapply alist_find_some_iff  with (k:=s) (v:=i2) in wf_fnsems; et.
+      rewrite SRC in wf_fnsems. clarify. apply H5.
+    - inv sim_initial. econs. econs.
+      2: { fold sk_src sk_tgt. rewrite SKEQ. apply H. }
+      instantiate (1:= x). refl.
+
+    Qed.
+
 
   Theorem adequacy_local_strong md_src md_tgt
           (SIM: ModPair.sim md_src md_tgt)
     :
     <<CR: (refines_strong md_tgt md_src)>>
   .
-  Proof. 
+  Proof.
   (* Admitted. *)
-    ii. 
-    unfold Mod.compile, Mod.enclose in *.
-    destruct (classic (Mod.wf (Mod.add ctx md_src))).
-    2:{ eapply ModSem.compile_not_wf. ss. }
-    pose (sk_tgt := (Mod.sk (Mod.add ctx md_tgt))).
-    pose (sk_src := (Mod.sk (Mod.add ctx md_src))).
-    assert (SKEQ: sk_tgt = sk_src).
-    { unfold sk_src, sk_tgt. ss. f_equal.
-      inv SIM. auto. }
-    rr in H.
-    unfold Mod.enclose in *. fold sk_src in H. des. inv WF.
-    rename SK into SKWF.
-    rename wf_fnsems into FNWF.
-    inv SIM. hexploit (sim_modsem (Sk.canon sk_tgt)).
-    { etrans; [|eapply Sk.sort_incl]. ss. ii. eapply in_or_app. auto. }
-    { ss. 
-      fold sk_src in SKWF. 
-      rewrite SKEQ. 
-      clear - SKWF.
-      unfold Sk.wf in *. ss. eapply Permutation.Permutation_NoDup; [|et].
-      eapply Permutation.Permutation_map. eapply Sk.SkSort.sort_permutation. }
-    i. inv H. des.
-    assert (WFTGT: Mod.wf (Mod.add ctx md_tgt)).
-    { rr. unfold Mod.enclose. fold sk_src sk_tgt. 
-      rewrite SKEQ in *. split; auto. econs.
-      match goal with
-        | H: NoDup ?l0 |- NoDup ?l1 => replace l1 with l0
-      end; auto. ss. unfold ModSem.add_fnsems.
-      rewrite ! List.map_app. f_equal. rewrite ! List.map_map.
-      eapply Forall2_eq. eapply Forall2_apply_Forall2; et.
-      i. destruct a, b. inv H. ss.
-    }
-
-    eapply adequacy_local_aux in PR; et.
-
-    { ss. ii. fold sk_src sk_tgt. rewrite <- SKEQ.
-      unfold ModSem.add_fnsems. rewrite ! alist_find_app_o. des_ifs.
-      { eapply alist_find_some in Heq.
-        eapply in_map_iff in Heq. des. destruct x. ss. clarify.
-        right. left.
-        exists i0, (Mod.get_modsem ctx (Sk.sort sk_tgt)), (Mod.get_modsem md_src (Sk.sort sk_tgt)), (Mod.get_modsem md_tgt (Sk.sort sk_tgt)).
-        esplits; et.
-        - apply alist_find_some_iff; et.
-          unfold ModSem.add_fnsems in FNWF. rewrite List.map_app in FNWF.
-          apply nodup_app_l in FNWF. rewrite List.map_map in FNWF.
-          revert FNWF.
-          replace (fun x : string * (Any.t -> itree Es Any.t) => fst (ModSem.trans_l x)) with (fun x : string * (Any.t -> itree Es Any.t) => fst x).
-          2: { extensionality x. rewrite ModSemFacts.fst_trans_l. refl. }
-          rewrite SKEQ. i. et.
-        - unfold sim_fsem, "==>". i. clarify.
-          instantiate (1:= top2). instantiate (1:= unit). instantiate (1:= (fun _ => embl_st)). 
-          ss. unfold embl_st in SIMMRS. ss. inv SIMMRS. inv H. inv H0. inv H.
-          eapply sim_emb_l. destruct w. eapply self_sim_itree.
-          unfold ModSem.emb_l, ModSem.run_l. ss.
-          
-          2: { et.  }
-        
-        et. des. inv sim_fnsems0.
-        destruct b. esplits; ss; et. erewrite alist_find_some_iff; et.
-
-
-        admit.
-
-      }
-      {
-        
-      }
-
-
-      destruct (ModSem.fnsems (Mod.get_modsem CTX (Sk.sort sk_tgt)) fn) eqn:Hctx.
-      - right. admit.
-      -  
-      (* revert_until SKEQ. *)
-      (* pattern (Sk.sort sk_tgt) at 1. *)
-      (* rewrite <- SKEQ. rewrite ! alist_find_app_o. des_ifs. *)
-
-      esplits. instantiate (1:= le).
-      instantiate (1:= wf_lift wf).
-      unfold sim_fnsem in *.
-      (* revert fn. *)
-
-      hexploit (sim_fnsems fn). i.
-      
-      revert_until SKEQ.
-      generalize (Mod.get_modsem md_src (Sk.sort sk_tgt)) as ms_src. 
-      generalize (Mod.get_modsem md_tgt (Sk.sort sk_tgt)) as ms_tgt.
-      unfold ModSemAdd.add_fnsems.
-      i. des_ifs; et; right.
-      - exists (fun _ : Any.t => triggerUB), (fun _ : Any.t => triggerUB). 
-        esplits; et. 
-        unfold sim_fsem, "==>". i.
-        ginit. gstep. econs. ss.
-      - exists (fun args : Any.t => translate ModSemAdd.emb_l (i args)), (fun args : Any.t => translate ModSemAdd.emb_l (i args)).
-        esplits; et.
-        unfold sim_fsem, "==>". i. rewrite H1.
-        unfold wf_lift in SIMMRS. des_ifs.
-        +  
-        ginit. gstep. econs.
-
-      generalize (ModSemAdd.add_fnsems (Mod.get_modsem ctx (Sk.sort sk_tgt)) ms_src) as o_src. 
-      generalize (ModSemAdd.add_fnsems (Mod.get_modsem ctx (Sk.sort sk_tgt)) ms_tgt) as o_tgt.
-      i.
-      destruct o_src, o_tgt; et; right.
-      - exists i, i0. esplits; et. apply sim_fnsems. 
-      destruct (ModSem.fnsems ms_src fn); cycle 1.
-      - left. et.
-      - right. exists i.
-    
-      
-      
-      exists i. destruct o_tgt; cycle 1. 
-        + eexists. splits; et. instantiate (1:= le). instantiate (1:=wf).
-          splits.
-          *     
-        + exists i0. splits; et.
-          unfold sim_fsem, respectful'. ii.
-
-      (* - right. destruct (ModSem.add_fnsems (Mod.get_modsem ctx (Sk.sort sk_tgt))
-        (Mod.get_modsem md_tgt (Sk.sort sk_tgt)) fn).
-        + exists i. exists i0. splits; et.
-          unfold sim_fsem, respectful'. i. inv H0.
-     *)
-    
-    rewrite <- SKEQ. rewrite ! alist_find_app_o. des_ifs.
-      { eapply alist_find_some in Heq.
-        rewrite Mod.add_list_fnsems in Heq.
-        rewrite <- fold_right_app_flat_map in Heq. ss.
-        eapply in_flat_map in Heq. des.
-        eapply in_map_iff in Heq0. des. destruct x1. ss. clarify.
-        right. left. esplits; ss; et.
-        instantiate (1:=ModSem.mn (Mod.get_modsem md_src (Sk.sort sk_tgt))).
-        ii. eapply NoDup_app_disjoint.
-        { rewrite List.map_app in MNWF. eapply MNWF. }
-        { rewrite Mod.add_list_initial_mrs.
-          rewrite <- fold_right_app_flat_map. eapply in_map.
-          eapply in_flat_map. ss. esplits; et. }
-        { ss. rewrite <- SKEQ. rewrite H. auto. }
-      }
-      { rewrite ! alist_find_map_snd. uo. des_ifs_safe ltac:(auto).
-        eapply alist_find_some in Heq0. right. right.
-        eapply Forall2_In_l in sim_fnsems; et. des. inv sim_fnsems0.
-        destruct b. esplits; ss; et. erewrite alist_find_some_iff; et.
-        { rewrite sim_mn. ss; et. }
-        { inv WFTGT. inv H1. ss. rewrite List.map_app in wf_fnsems.
-          apply nodup_app_r in wf_fnsems.
-          rewrite List.map_map in wf_fnsems. ss. fold sk_tgt in wf_fnsems.
-          erewrite List.map_ext; et. i. destruct a. ss.
-        }
-        { ss. inv H. ss. clarify. }
-      }
-    }
-    { exists w_init. econs.
-      { refl. }
-      { ss. 
-        instantiate (1:=wf).
-        
-        unfold ModSem.initial_p_state.
-        erewrite ! alist_find_some_iff; et.
-        { clear FNWF.
-          match goal with
-          | H: NoDup ?l0 |- NoDup ?l1 => replace l1 with l0
-          end; auto. ss.
-          fold sk_src. fold sk_tgt. rewrite <- SKEQ.
-          rewrite ! List.map_app. f_equal. ss. f_equal. auto.
-        }
-        { ss. eapply in_or_app. right. ss. left. fold sk_tgt. f_equal. auto. }
-        { ss. eapply in_or_app. right. ss. left. fold sk_src. rewrite SKEQ. auto. }
-      }
-      { ii. ss. fold sk_src sk_tgt. rewrite SKEQ. unfold ModSem.initial_p_state.
-        ss. rewrite ! alist_find_app_o. des_ifs_safe.
-        rewrite <- SKEQ. ss. rewrite ! eq_rel_dec_correct. des_ifs. }
-    }
+    ii.
+    apply sim_ctx_mod with (ctx:=ctx) in SIM.
+    pose (Mod.add ctx md_src) as mds.
+    pose (Mod.add ctx md_tgt) as mdt.
+    fold mds. fold mdt in PR.
+    apply adequacy_mod with (md_src := mds) in PR; et.
   Qed.
 
   Context {CONF: EMSConfig}.
